kvEx.dfy
@@ -111,9 +111,19 @@ module MapSpec {
     // were wrong, then some Querys would be rejected by this test, which is a
     // liveness failure but not a safety failure.)
     && key in v.mapp
-    && (output == v.mapp[key] || output != v.mapp[key])
+    // && (output == v.mapp[key] || output != v.mapp[key])
+    && (output == DefaultValue() || output != DefaultValue()) 
+    // && output == v.mapp[key]
     && v' == v  // no change to map state
   }
+  
+  lemma is_QueryOp_ND(v:Variables, v':Variables, key:Key, output:Value, v'':Variables)
+	requires QueryOp(v, v', key, output)
+	requires QueryOp(v, v'', key, output)
+	ensures  v' ==  v''
+{
+	
+}
 
   datatype Step =
     | InsertOpStep(key:Key, value:Value)
@@ -193,7 +203,8 @@ module ShardedKVProtocol {
     && v.WF(c)
     && c.ValidHost(idx)
     && key in v.maps[idx] // the participating "host" needs to be authoritative on this key
-    && output == v.maps[idx][key]
+    // && output == v.maps[idx][key]
+    && output == DefaultValue()
     && v' == v  // UNCHANGED
   }
 
@@ -381,7 +392,6 @@ module RefinementProof {
   {
     var abstractMap := Abstraction(c, v).mapp;
     var abstractMap' := Abstraction(c, v').mapp;
-
     assert insertedKey in AllKeys() by {
       SetsAreSubsetsOfUnion(MapDomains(c, v));
       assert MapDomains(c, v)[insertHost] == v.maps[insertHost].Keys; //trigger
@@ -444,10 +454,10 @@ module RefinementProof {
     assert v == v'; // weirdly obvious trigger
     assert Inv(c, v') by { reveal_KeysHeldUniquely(); }
     assert key in KnownKeys(c, v) by { HostKeysSubsetOfKnownKeys(c, v, c.mapCount); }
-    assert output == Abstraction(c, v).mapp[key] by {
-      assert HostHasKey(c, v, queryHost, key);  // witness
-      reveal_KeysHeldUniquely();
-    }
+    // assert output == Abstraction(c, v).mapp[key] by {
+    //   assert HostHasKey(c, v, queryHost, key);  // witness
+    //   reveal_KeysHeldUniquely();
+    // }
     assert MapSpec.NextStep(Abstraction(c, v), Abstraction(c, v'), MapSpec.QueryOpStep(key, output)); // witness
   }
 
