README.md
@@ -2,18 +2,20 @@ Work in progress for automation tools for spec testing.
 
 Files:
 
-* mutationEx.dfy : example for mutation testing prototype
+* maxPredMutation.dfy : example for mutation testing prototype (incorrect Spec)
+* correctMaxPredMutation.dfy : example for mutation testing prototype (correct Spec)
+* kvEx.dfy : Key Value refinement proof
 * specMutationTest.s.dfy : example of manual muation testing. 
-* template.s.dfy : Examples for ND testing 
+* template.s.dfy : Examples for Non-Deterministic testing 
 * specTest.s.dfy : More manual tests 
 
-See `/.scripts` for more details about Fuzzing and Non-Deterministic Testing
+See `/.scripts` for more details and documentation about Fuzzing and Non-Deterministic Testing
 
 ---
 
 ### Mutation Testing Prototype
 
-Starting with a Spec, and a proof that passes, running a mutating the spec and retrying the proof gives an indication that the spec could be too weak. If a stronger mutated spec still allows the proof to go through, this is a red flag, that the original spec may not be the intended spec. 
+Starting with a Spec, and a proof that passes, running a mutatation of the spec and having  the proof pass gives an indication that the spec could be too weak. If a non-weaker mutated spec still allows the proof to go through, this is a red flag, that the original spec may not be the intended spec. 
 
 https://github.com/eligoldweber/dafny-holeEval/tree/mutations
 
@@ -31,7 +33,9 @@ To run:
 ./Binaries/Dafny /rlimit:1000 /compile:0 /allowGlobals /noNLarith /autoTriggers:1 /verifyAllModules /holeEval:[MODULE_NAME].[PREDICATE NAME] /proofName:[MODULE_NAME].[PREDICATE NAME] /holeEvalRunOnce /holeEvalServerIpPortList:ipPortListOneNode.txt [PATH TO FILE].dfy &> output.txt
 ```
 
-By including the `/proofName` commandline parameter, this tool will automatically check for each mutation in order, if the mutation is Stronger without the proof, if the mutation is equivalent to the un-mutated predicate without the proof, and finally if the first two checks pass, will check if the proof still passes with the mutation. 
+By including the `/proofName` commandline parameter, this tool will only check the mutated spec with the full proof if it pases some pre-processing steps that determine if the spec is strictly not weaker or eqaul to the original spec.
+
+Include `/proofModuleName` if the proof is containted in a different module. In this case the tool will comment out this entire module when doing pre-processing. This module must be the last module in the file. Additionally, all needed modules (ie. `import opened module`) must be in the same file. 
 
 See `correctMaxPredMutation.dfy`, and `maxPredMutation.dfy` for example files;
 
@@ -41,16 +45,20 @@ for example:
 ./Binaries/Dafny /rlimit:1000 /compile:0  /allowGlobals /noNLarith /autoTriggers:1 /verifyAllModules /holeEval:maxExample.maxSpec /proofName:maxExample.max /holeEvalRunOnce /holeEvalServerIpPortList:ipPortListOneNode.txt ~/maxPredMutation.dfy &> output.txt
 ```
 
+KV mutation example: 
+
+```
+./Binaries/Dafny /compile:0 /timeLimit:60 /trace /arith:5 /noCheating:1 /holeEval:MapSpec.QueryOp /proofName:RefinementProof.RefinementNext /proofModuleName:RefinementProof /holeEvalRunOnce /holeEvalServerIpPortList:PortListOneNode.txt ~/counterExampleTest/specTesting/kvEx.dfy &> output.txt
+```
+
 The output from this tool will generate a log in `output.txt` and will display all the attempted mutations, and the ones that passed. As well
 as a directory of intermediary files. 
 
-The `isStronger` lemma checks to see if the mutated predicate is stronger than the original predicate. We dont care about weaker mutations. 
-It is possible for a mutation to be exactly the same as the original predicate, which will lead to a false positive. The same predicate will also
-allow the proof to pass. Avoid this by checking which of the mutations are equal. A TODO is to check this programatically so to only run the proof with
-the mutations that are valid. unique and stronger. 
+There are 2 prepocessing steps `isWeaker` lemma checks to see if the mutated predicate is weaker than the original predicate. We dont care about weaker mutations. 
+It is possible for a mutation to be exactly the same as the original predicate, which will lead to a false positive. The next check fixes this by checking which of the mutations are equal. 
 
 
->NOTE: an example for the body of the ipPortListOneNode.txt file is `[IP]:50051` for running both the holeEval tool and the grpc server on the same host. The default port configured for the dafny-grpc-server is 50051. Both the dafny server and holeEval tool can be run on the same machine, but it is suggested to at least use multiple sessions. 
+>NOTE: an example for the body of the ipPortListOneNode.txt file is just `[IP]:50051` for running both the holeEval tool and the grpc server on the same host. The default port configured for the dafny-grpc-server is 50051. Both the dafny server and holeEval tool can be run on the same machine, but it is suggested to at least use multiple sessions. 
 
 https://github.com/arminvakil/dafny-grpc-server
 
